Rebase of the fundamental branch of Loïc

theories/LogicalRelation/Universe.v
@@ -1,11 +1,74 @@
-From LogRel.AutoSubst Require Import core unscoped Ast Extra.
-From LogRel Require Import Utils BasicAst Context Untyped Weakening GenericTyping LogicalRelation Reduction.
-From LogRel.LogicalRelation Require Import Irrelevance Induction.
+From LogRel.AutoSubst Require Import core unscoped Ast.
+From LogRel Require Import Utils BasicAst Notations Context Untyped Weakening GenericTyping LogicalRelation.
+From LogRel.LogicalRelation Require Import Induction Escape Irrelevance.
 
 Set Universe Polymorphism.
+Set Printing Universes.
 
-Section Universe.
+Section UniverseReducibility.
   Context `{GenericTypingProperties}.
+
+  (* These proofs are somewhat hack-ish and do not generalize properly to arbitrarily many universes *)
+  (* In particular, they exploit the following lemma, which proves "cumulativity" of LogRel0, but
+     unfortunately this lemma does not generalize to LogRel l *)
+  (* In proper generality, one would need to show that
+     LogRel@{i j k} l Γ A EqTy RedTm EqTm -> LogRel@{j k l} l Γ A EqTy' RedTm' EqTm'
+     where EqTy' RedTm' EqTm' are equivalent but non definitionally equal predicates *)
+
+  Definition LogRel0_Cumulative@{i j k l} {Γ A} {EqTy RedTm : term -> Type@{j}} {EqTm : term -> term -> Type@{j}}
+    (lr : LogRel0@{i j k} Γ A EqTy RedTm EqTm) : LogRel0@{j k l} Γ A EqTy RedTm EqTm.
+  Proof.
+    induction lr as [ ? HU | ? ? neA | ? ? ? ? domAd codAd ].
+    - exact (match elim HU.(URedTy.lt) with end).
+    - exact (LRne _ neA).
+    - eapply LRPi@{j k l}. unshelve econstructor.
+      + exact domAd.
+      + exact codAd.
+  Defined.
+
+  Definition TyRed_Cumulative@{i j k l} {Γ} {A} (rA : [ LogRel0@{i j k} | Γ ||- A ])
+      : [ LogRel0@{j k l} | Γ ||- A ].
+  Proof.
+    destruct rA as [Pack PackAd].
+    unshelve econstructor.
+    - exact Pack.
+    - exact (LogRel0_Cumulative@{i j k l} PackAd).
+  Defined.
+
+  Lemma redUOne {Γ l A} : [Γ ||-<l> A] -> [Γ ||-U one].
+  Proof.
+    intros ?%escape_; econstructor; [easy| gen_typing].
+  Qed.
+
+  Lemma UnivEq'@{i j k l} {Γ A l} (rU : [ LogRel@{i j k l} l | Γ ||- U ]) (rA : [ LogRel@{i j k l} l | Γ ||- A : U | rU])
+    : [ LogRel@{i j k l} zero | Γ ||- A].
+  Proof.
+    assert [ LogRel@{i j k l} one | Γ ||- A : U | LRU_@{i j k l} (redUOne rU)]
+             as [ _ _ _ _ hA ] by irrelevance.
+    exact (TyRed_Cumulative hA).
+  Defined.
+
+  Lemma UnivEq@{i j k l} {Γ A l} l' (rU : [ LogRel@{i j k l} l | Γ ||- U]) (rA : [ LogRel@{i j k l} l | Γ ||- A : U | rU])
+    : [ LogRel@{i j k l} l' | Γ ||- A].
+  Proof.
+    destruct l'.
+    - eapply (UnivEq' rU rA).
+    - econstructor. eapply LR_embedding.
+      + exact Oi.
+      + apply (UnivEq' rU rA).
+  Defined.
+
+  Lemma UnivEqEq@{i j k l} {Γ A B l l'} (rU : [ LogRel@{i j k l} l | Γ ||- U ]) (rA : [LogRel@{i j k l} l' | Γ ||- A ]) (rAB : [ LogRel@{i j k l} l | Γ ||- A ≅ B : U | rU ])
+    : [ LogRel@{i j k l} l' | Γ ||- A ≅ B | rA ].
+  Proof.
+    assert [ LogRel@{i j k l} one | Γ ||- A ≅ B : U | LRU_@{i j k l} (redUOne rU) ] as [ _ _ _ hA _ hAB ] by irrelevance.
+    change ([ TyRed_Cumulative@{i j k l} hA | Γ ||- A ≅ B ]) in hAB.
+    eapply LRTyEqIrrelevant. exact hAB.
+  Qed.
+
+
+  (* The lemmas below does not seem to be
+     at the right levels for fundamental lemma ! *)
 
   Set Printing Universes.
   Lemma univTmTy'@{h i j k l} {Γ l A} (h : [Γ ||-U l]) :
@@ -29,6 +92,4 @@ Section Universe.
     [LogRel@{h i j k} l' | Γ ||- A ≅ B | RA].
   Proof. intros h; eapply (univEqTmEqTy' (invLRU RU)); irrelevance. Qed.
 
-End Universe.
-
-    
+End UniverseReducibility.
