theories/Fundamental.v
@@ -1,20 +1,20 @@
 From LogRel.AutoSubst Require Import core unscoped Ast Extra.
-From LogRel Require Import Utils BasicAst Notations Context Untyped Weakening 
-  DeclarativeTyping GenericTyping LogicalRelation
-  Validity.
-From LogRel.LogicalRelation Require Import Irrelevance Escape.
-From LogRel.Substitution Require Import Properties Irrelevance.
+From LogRel Require Import Utils BasicAst Notations Context Untyped Weakening
+  DeclarativeTyping GenericTyping LogicalRelation Validity.
+From LogRel.LogicalRelation Require Import Irrelevance Escape Reflexivity Universe Weakening.
+From LogRel.Substitution Require Import Irrelevance Properties.
 
 Set Primitive Projections.
 Set Universe Polymorphism.
+Set Polymorphic Inductive Cumulativity.
 
-(* FundCon, FundTy, ... are parameterized by a tag with a bunch of typing 
+(* FundCon, FundTy, ... are parameterized by a tag with a bunch of typing
   judgment predicates *)
 Definition FundCon `{GenericTypingProperties}
   (Γ : context) : Type := [||-v Γ ].
 
 Module FundTy.
-  Record FundTy `{GenericTypingProperties} {Γ : context} {A : term} 
+  Record FundTy `{GenericTypingProperties} {Γ : context} {A : term}
   : Type := {
     VΓ : [||-v Γ ];
     VA : [ Γ ||-v< one > A | VΓ ]
@@ -94,11 +94,69 @@ End FundSubstConv.
 Export FundSubstConv(FundSubstConv,Build_FundSubstConv).
 
 Section Fundamental.
-  (* Fundamental is parameterized by a tag that satisfies the generic typing 
+  (* Fundamental is parameterized by a tag that satisfies the generic typing
     properties *)
   Context `{GenericTypingProperties}.
-  (* On top of this, we need to use the predicates for declarative typing,
-    since we will reason by induction on them *)
+
+  Lemma TypeRedWf_refl {Γ} {A} : [ Γ |-[ ta ] A ] -> [ Γ |-[ ta ] A :⇒*: A ].
+  Proof.
+    intro h. econstructor.
+    - assumption.
+    - assumption.
+    - now apply redty_refl.
+  Defined.
+
+  Lemma ughhh {a σ ρ} : (tRel 1)[a .: σ⟨ρ⟩] = (tRel 1)[up_term_term σ][a .: ρ >> tRel].
+  Proof.
+    asimpl. Fail reflexivity.
+  Abort.
+
+  Lemma FundPi {l Γ na F G} (vΓ : [||-v Γ])
+    (vF : [Γ ||-v< l > F | vΓ])
+    (vG : [Γ ,, vass na F ||-v< l > G | validSnoc na vΓ vF])
+    : [Γ ||-v< l > tProd na F G | vΓ].
+  Proof.
+    pose proof (rF := fun Δ σ => validTy (Δ := Δ) (σ := σ) vF).
+    pose proof (tF := fun Δ σ tΔ vσ => escape_ (rF Δ σ tΔ vσ)).
+    pose proof (tFrefl := fun Δ σ tΔ vσ => escapeEq_ _ (LRTyEqRefl_ (rF Δ σ tΔ vσ))).
+    pose proof (rG := fun Δ σ tΔ vσ => validTy (Δ := Δ ,, vass na F[σ])
+                                         (σ := up_term_term σ) vG _ (liftSubstS' vΓ tΔ vF vσ)).
+    pose proof (tG := fun Δ σ tΔ vσ => escape_ (rG Δ σ tΔ vσ)).
+    pose proof (tGrefl := fun Δ σ tΔ vσ => escapeEq_ _ (LRTyEqRefl_ (rG Δ σ tΔ vσ))).
+    pose proof (rGa := fun Δ Δ' σ a (tΔ : [ |-[ ta ] Δ ]) (tΔ' : [ |-[ ta ] Δ' ]) ρ vσ ra =>
+                         validTy (Δ := Δ') (σ := a .: (σ ⟨ ρ ⟩)) vG _
+                           (consSubstS vΓ tΔ' (wkSubstS vΓ tΔ tΔ' ρ vσ) vF ra)).
+    unshelve econstructor.
+    - intros Δ σ tΔ vσ. cbn.
+      unshelve eapply LRPi_.
+      + econstructor.
+        * apply TypeRedWf_refl.
+          exact (wft_prod (tF _ _ tΔ vσ) (tG _ _ tΔ vσ)).
+        * exact (tF _ _ tΔ vσ).
+        * exact (tG _ _ tΔ vσ).
+        * exact (convty_prod I (tF _ _ tΔ vσ) (tFrefl _ _ tΔ vσ) (tGrefl _ _ tΔ vσ)).
+
+          Unshelve.
+          ++ intros Δ' ρ tΔ'.
+             exact (wk ρ tΔ' (rF Δ σ tΔ vσ)).
+          ++ intros Δ' a ρ tΔ' ra.
+            admit.
+
+        * intros Δ' a b ρ tΔ' ra rb rab.
+          admit.
+
+      + econstructor.
+        * fold subst_term. admit.
+        * admit.
+    - intros Δ σ σ' tΔ vσ vσ' vσσ'. simpl. fold subst_term.
+      econstructor.
+      + apply TypeRedWf_refl.
+        exact (wft_prod (tF _ _ tΔ vσ') (tG _ _ tΔ vσ')).
+      + fold subst_term. simpl. admit.
+      + fold subst_term. simpl. admit.
+      + fold subst_term. simpl. admit.
+  Admitted.
+
   Import DeclarativeTypingData.
 
   Lemma FundConNil : FundCon ε.
@@ -110,27 +168,45 @@ Section Fundamental.
   + constructor.
   Qed.
 
-  Lemma FundConCons : forall (Γ : context) (na : aname) (A : term),
-  [ |-[ de ] Γ] -> FundCon Γ -> [Γ |-[ de ] A] -> FundTy Γ A -> FundCon (Γ,, vass na A).
+  Lemma FundConCons (Γ : context) (na : aname) (A : term)
+  (tΓ : [ |-[ de ] Γ]) (fΓ : FundCon Γ) (tA : [Γ |-[ de ] A]) (fA : FundTy Γ A) : FundCon (Γ,, vass na A).
   Proof.
-  Admitted.
+    destruct fA as [ vΓ vA ].
+    eapply validSnoc. exact vA.
+  Qed.
 
-  Lemma FundTyU : forall (Γ : context),
-    [ |-[ de ] Γ] -> FundCon Γ -> FundTy Γ U.
+  Lemma FundTyU (Γ : context) (tΓ : [ |-[ de ] Γ]) (fΓ : FundCon Γ) : FundTy Γ U.
   Proof.
-  Admitted.
+    unshelve econstructor.
+    - assumption.
+    - unshelve econstructor.
+      + intros * _. apply LRU_. now econstructor.
+      + intros * _ _. simpl. now econstructor.
+  Qed.
 
-  Lemma FundTyPi : forall (Γ : context) (na : aname) (A B : term),
-    [Γ |-[ de ] A] -> FundTy Γ A ->
-    [Γ,, vass na A |-[ de ] B] -> FundTy (Γ,, vass na A) B ->
-    FundTy Γ (tProd na A B).
+  Lemma FundTyPi (Γ : context) (na : aname) (F G : term)
+    (tF : [Γ |-[ de ] F]) (fF : FundTy Γ F)
+    (tG : [Γ,, vass na F |-[ de ] G]) (fG : FundTy (Γ,, vass na F) G)
+    : FundTy Γ (tProd na F G).
   Proof.
-  Admitted.
+    destruct fF as [ vΓ vF ]. destruct fG as [ vΓF vG ].
+    econstructor.
+    unshelve eapply (FundPi vΓ).
+    - assumption.
+    - now eapply irrelevanceValidity.
+  Qed.
 
-  Lemma FundTyUniv : forall (Γ : context) (A : term),
-    [Γ |-[ de ] A : U] -> FundTm Γ U A -> FundTy Γ A.
+  Lemma FundTyUniv (Γ : context) (A : term)
+    (tA : [Γ |-[ de ] A : U]) (fA : FundTm Γ U A)
+    : FundTy Γ A.
   Proof.
-  Admitted.
+    destruct fA as [ vΓ vU [ rA rAext ] ]. econstructor.
+    unshelve econstructor.
+    - intros * vσ.
+      eapply UnivEq. exact (rA _ _ wfΔ vσ).
+    - intros * vσ' vσσ'.
+      eapply UnivEqEq. exact (rAext _ _ _ wfΔ vσ vσ' vσσ').
+  Qed.
 
   Lemma FundTmVar : forall (Γ : context) (n : nat) (decl : context_decl),
     [ |-[ de ] Γ] -> FundCon Γ ->
